Using Trans in Relations.

src/part1/Relations.lean
@@ -2,94 +2,49 @@ open Nat
 
 namespace Relations
 
-inductive True : Prop where
-| tt : True
-
-inductive False : Prop where
--- this line deliberately left blank
-
-theorem ex_quod_libet : ∀ (P : Prop), False → P
-  := by
-       intros P f
-       cases f
-
-
 inductive le : Nat → Nat → Prop
 | refl : ∀ {m}, le m m
 | step : ∀ {m n}, le m n → le m (succ n)
 
-open le
-
 instance : LE Nat where
   le := le
+
+theorem trans_le : ∀ {m n p : Nat}, m ≤ n → n ≤ p → m ≤ p
+  := by
+       intros m n p m_le_n n_le_p
+       induction n_le_p with
+       | refl => assumption
+       | step _ ih => apply le.step; exact ih
+
+instance : Trans (.≤. : Nat → Nat → Prop)
+                 (.≤. : Nat → Nat → Prop)
+                 (.≤. : Nat → Nat → Prop) where
+  trans := trans_le
+
+example : 2 ≤ 7 :=
+  calc
+    2 ≤ 4 := le.step (le.step le.refl)
+    _ ≤ 5 := le.step le.refl 
+    _ ≤ 7 := le.step (le.step le.refl)
 
 def lt (n m : Nat) := le (succ n) m
 
 instance : LT Nat where
   lt := lt
 
-theorem invert : ∀ {m n : Nat}, succ m ≤ succ n -> m ≤ n
+def invert : ∀ {m n : Nat}, succ m ≤ succ n -> m ≤ n
   := by
-      intros m n sm_le_sn
-      cases sm_le_sn with
+      intros m n m_le_n
+      cases m_le_n with
       | refl =>
-         exact refl
-      | step sm_le_n =>
-         cases n with
-         | zero => contradiction
-         | succ n => apply step; apply invert; assumption
+         exact le.refl
+      | step m_le_n =>
+        cases n with
+        | zero => contradiction
+        | succ n => apply le.step; apply invert; assumption
 
 -- Proof is by induction, but induction tactic does not apply.
 -- Note explicit application of "invert"
-
-def trans_le : ∀ {m n p : Nat}, m ≤ n → n ≤ p → m ≤ p
-  := by
-       intros m n p m_le_n n_le_p
-       induction n_le_p with
-       | refl => assumption
-       | step n_le_p ih => apply step; exact ih
-
-example : 2 ≤ 5 := step (step (step refl))
---  calc
---    2 ≤ 2  := refl
---    _ ≤ 3  := step _
-
--- Exercise.
--- Here is a different definition of ≤.
--- Prove the two definitions equivalent,
--- that is, that each implies the other.
-
-inductive le2 : Nat → Nat → Prop
-| z_le_n :
-      ----------
-      le2 zero n
-| s_le_s :
-      le2 m n
-      ---------------------
-    → le2 (succ m) (succ n)
-
-open le2
-
--- Exercise.
--- Prove lt, lt2, and lt3 equivalent.
-
-inductive lt2 : Nat → Nat → Prop where
-| z_lt_s : ∀ {n}, lt2 zero (succ n)
-| s_lt_s : ∀ {m n},
-      lt2 m n
-      ---------------------
-    → lt2 (succ m) (succ n)
-
-inductive lt3 : Nat → Nat → Prop where
-| m_lt_sm : ∀ {m}, lt3 m (succ m)
-| m_lt_sn : ∀ {m n},
-      lt3 m n
-      ---------------------
-    → lt3 m (succ n)
-
--- Exercise. Prove the following.
---   m ≤ n iff ∃ p, m + p = n
---   m < n iff ∃ p, p ≠ 0 ∧ m + p = n
 
 
 
